src/PlutusIR/Cert/Claim.v
@@ -6,79 +6,94 @@ From PlutusCert Require Import
   SemanticEquivalence.Contextual
 .
 
-Inductive claim :=
-  | Verified : rel_verified -> claim
-  | Related  : rel_decidable -> claim
-  | Unknown  : claim
-.
-
-Definition claim_prop : claim -> (term -> term -> Prop) := fun c t t' =>
-  match c with
-  | Verified rv => forall Δ Γ T, Δ ,, Γ |- t ≃-ctx t' : T
-  | Related rd  => rd_rel rd t t'
-  | Unknown     => True
-  end
-.
-
-Definition claim_decb : claim -> (term -> term -> bool) := fun c =>
-  match c with
-  | Verified rv => rd_decb (rv_rd rv)
-  | Related rd  => rd_decb rd
-  | Unknown     => fun t t' => true
-  end
-.
-
-Definition claim_decb_eq (c : claim) (t t' : term) : option (claim_decb c t t' = true)
-  := match claim_decb c t t' with
-    | true  => Some eq_refl
-    | false => None
-  end.
-
-Definition claim_dec (c : claim) (t t' : term) : option (claim_prop c t t') :=
-  match c return option (claim_prop c t t') with
-    | Verified rv => rv_dec rv t t'
-    | Related rd  => rd_dec rd t t'
-    | Unknown     => Some I
-  end
-.
-
-
 Require Import Lists.List.
 Import ListNotations.
 
-(* Deciding trace claims *)
+Section Claims.
 
-Fixpoint trace_prop' (ps : list (pass * term)) : forall (claims : pass -> claim) (t : term), Prop :=
-    fun claims t => match ps with
-      | [] => True
-      | (p, t') :: ps => claim_prop (claims p) t t' /\ trace_prop' ps claims t'
+  Inductive claim :=
+    | Unchecked : claim
+    | AccordingToSpec  : rel_decidable -> claim
+    | Verified : rel_verified -> claim
+  .
+
+  (* Interpret a claim as a Prop on terms *)
+  Definition claim_prop : claim -> (term -> term -> Prop) := fun c t t' =>
+    match c with
+    | Verified rv => forall Δ Γ T, Δ ,, Γ |- t ≃-ctx t' : T
+    | AccordingToSpec rd  => rd_rel rd t t'
+    | Unchecked     => True
+    end
+  .
+
+  Definition claim_decb : claim -> (term -> term -> bool) := fun c =>
+    match c with
+    | Verified rv => rd_decb (rv_rd rv)
+    | AccordingToSpec rd  => rd_decb rd
+    | Unchecked     => fun t t' => true
+    end
+  .
+
+  Definition claim_decb_eq (c : claim) (t t' : term) : option (claim_decb c t t' = true)
+    := match claim_decb c t t' with
+      | true  => Some eq_refl
+      | false => None
     end.
 
-Definition trace_prop : (pass -> claim) -> compilation_trace -> Prop :=
-  fun claims ct =>
-  match ct with
-  | CompilationTrace t0 ps => trace_prop' ps claims t0
-  end.
+  Definition claim_dec (c : claim) (t t' : term) : option (claim_prop c t t') :=
+    match c return option (claim_prop c t t') with
+      | Verified rv => rv_dec rv t t'
+      | AccordingToSpec rd  => rd_dec rd t t'
+      | Unchecked     => Some I
+    end
+  .
 
-Fixpoint trace_dec' (claims : pass -> claim) (t : term) (ps : list (pass * term))
-  : option (trace_prop' ps claims t) :=
-  match ps return option (trace_prop' ps claims t) with
-  | [] => Some I
-  | (p, t') :: ps =>
-    match claim_dec (claims p) t t' with
-    | Some proof =>
-      match trace_dec' claims t' ps with
-      | Some proofs => Some (conj proof proofs)
+  Fixpoint claims_prop' (ps : list (pass * term)) :
+    (pass -> claim) -> term -> Prop :=
+      fun claims t_pre => match ps with
+        | [] => True
+        | (p, t_post) :: ps => claim_prop (claims p) t_pre t_post /\ claims_prop' ps claims t_post
+      end.
+
+  Definition claims_prop : (pass -> claim) -> compilation_trace -> Prop :=
+    fun claims ct =>
+    match ct with
+    | CompilationTrace t0 ps => claims_prop' ps claims t0
+    end.
+
+  Fixpoint trace_dec' (claims : pass -> claim) (t : term) (ps : list (pass * term))
+    : option (claims_prop' ps claims t) :=
+    match ps return option (claims_prop' ps claims t) with
+    | [] => Some I
+    | (p, t') :: ps =>
+      match claim_dec (claims p) t t' with
+      | Some proof =>
+        match trace_dec' claims t' ps with
+        | Some proofs => Some (conj proof proofs)
+        | None => None
+        end
       | None => None
       end
-    | None => None
     end
-  end
-.
+  .
 
-Definition trace_dec (claims : pass -> claim) (ct : compilation_trace)
-  : option (trace_prop claims ct) :=
-  match ct with
-  | CompilationTrace t0 ps => trace_dec' claims t0 ps
+  Definition trace_dec (claims : pass -> claim) (ct : compilation_trace)
+    : option (claims_prop claims ct) :=
+    match ct with
+    | CompilationTrace t0 ps => trace_dec' claims t0 ps
+    end
+  .
+
+End Claims.
+
+
+
+Definition default_claims : pass -> claim := fun p =>
+  match p with
+  | PassTypeCheck => AccordingToSpec rd_equal
+  (* | PassRename    => AccordingToSpec rd_rename *)
+  | PassDeadCode  => AccordingToSpec rd_deadcode
+  | PassCompileLetNonRec => Verified let_nonrec
+  | _             => Unchecked
   end
 .
