src/PlutusIR/Cert/Relation/DeadCode.v
@@ -4,9 +4,10 @@ From PlutusCert Require Import
   DeadCode.DecideBool
 .
 
+
 Definition rd_deadcode : rel_decidable :=
   mk_rel_decidable
     elim
-    dec_Term
-    dec_Term_equiv
+    dec_Term'
+    dec_Term'_equiv
 .
